src/CDCL/Spec.v
@@ -251,7 +251,8 @@ Definition staged_invariant (work : list ClauseId) (s : State) : Prop :=
   /\ (forall ci, In ci work ->
      card_of_watch work ci s = 1 \/
      (card_of_watch work ci s = 0 /\
-       exists l, In (l, ci) s.(state_pending)))
+       ((exists l, In (l, ci) s.(state_pending)) \/
+        decided_clause ci s)))
   /\ (forall ci,
      card_of_watch work ci s = 0 \/
      card_of_watch work ci s = 2 \/
@@ -453,10 +454,12 @@ Proof.
            ++ intros d. destruct (Nat.eq_dec ci d) as [->|Hneq].
               ** unfold card_of_watch. cbn -[ClauseMap.card_of].
                  rewrite ClauseMap.card_of_add.
-                 destruct Hciwork as [Hone|[Hzero [p Hpendingci]]].
+                 destruct Hciwork as [Hone|[Hzero [[p Hpendingci]|Hdecided]]].
                  --- rewrite Hone. now right; left.
                  --- rewrite Hzero. right; right. split; [reflexivity|].
                      right. left. now exists p.
+                 --- rewrite Hzero. right; right. split; [reflexivity|].
+                     right. right. exact Hdecided.
               ** specialize (Hcard d).
                  unfold card_of_watch in Hcard |- *. cbn -[ClauseMap.card_of].
                  rewrite ClauseMap.card_of_add_neq by exact Hneq.
@@ -523,9 +526,10 @@ Proof.
     + injection Heq as <- <-. exists c. repeat split; try assumption. now left.
     + exact (Hpending p d Hpd).
   - intros d Hd. specialize (Hwork d Hd).
-    destruct Hwork as [Hone|[Hzero [p Hpd]]].
+    destruct Hwork as [Hone|[Hzero [[p Hpd]|Hdecided]]].
     + now left.
-    + right. split; [exact Hzero|]. exists p. now right.
+    + right. split; [exact Hzero|]. left. exists p. now right.
+    + right. split; [exact Hzero|]. right. exact Hdecided.
   - intros d. specialize (Hcard d).
     destruct Hcard as [Hzero|[Htwo|[Hone Hwhy]]].
     + now left.
@@ -568,9 +572,10 @@ Proof.
       * injection Heq as <- <-. exists c. repeat split; try assumption. now left.
       * exact (Hpending p d Hpd).
     + intros d Hd. specialize (Hwork d (or_intror Hd)).
-      destruct Hwork as [Hone|[Hzero [p Hpd]]].
+      destruct Hwork as [Hone|[Hzero [[p Hpd]|Hdecided]]].
       * now left.
-      * right. split; [exact Hzero|]. exists p. now right.
+      * right. split; [exact Hzero|]. left. exists p. now right.
+      * right. split; [exact Hzero|]. right. exact Hdecided.
     + intros d. specialize (Hcard d).
       destruct Hcard as [Hzero|[Htwo|[Hone Hwhy]]].
       * now left.
@@ -628,7 +633,11 @@ Proof.
     + now right; left.
     + right. right. now apply Hfalspreserve.
   - intros d Hd. exact (Hworkref d (or_intror Hd)).
-  - intros d Hd. exact (Hwork d (or_intror Hd)).
+  - intros d Hd. specialize (Hwork d (or_intror Hd)).
+    destruct Hwork as [Hone|[Hzero [Hpendingd|Hdecided']]].
+    + now left.
+    + right. split; [exact Hzero|]. now left.
+    + right. split; [exact Hzero|]. right. now apply Hdecided.
   - intros d. specialize (Hcard d).
     destruct Hcard as [Hzero|[Htwo|[Hone Hwhy]]].
     + now left.
@@ -709,4 +718,467 @@ Lemma fold_propagate_inv : forall work s,
 Proof.
   induction work as [|ci work IH]; intros s Hinv; [exact Hinv|].
   simpl. apply IH. now apply propagate_inv.
+Qed.
+
+Lemma prepare_set_lit_inv : forall l m clauses cm fals pending,
+  literal_is_undecided m l = true ->
+  state_invariant
+    {| state_model := m; state_clauses := clauses; state_watched := cm;
+       state_falsified := fals; state_pending := pending |} ->
+  staged_invariant (ClauseMap.find (literal_var l) cm)
+    {| state_model := l :: m; state_clauses := clauses;
+       state_watched := ClauseMap.remove (literal_var l) cm;
+       state_falsified := fals; state_pending := pending |}.
+Proof.
+  intros l m clauses cm fals pending Hlu Hinv.
+  destruct Hinv as
+    [Hcover [Hfals [Hwatch [Hnodup [_ [_ [Hpending [_ Hcard]]]]]]]].
+  assert (Hdecided : forall d,
+      decided_clause d
+        {| state_model := m; state_clauses := clauses; state_watched := cm;
+           state_falsified := fals; state_pending := pending |} ->
+      decided_clause d
+        {| state_model := l :: m; state_clauses := clauses;
+           state_watched := ClauseMap.remove (literal_var l) cm;
+           state_falsified := fals; state_pending := pending |}).
+  { intros d [Hd|[body [Hbody Htrue]]].
+    - now left.
+    - right. exists body. split; [exact Hbody|].
+      now apply satisfied_cons_undecided. }
+  repeat split.
+  - intros d body Hbody Hfalse.
+    assert (Holdfalse :
+      Is_true (negb (existsb (literal_is_true m) body))).
+    { apply negb_prop_intro. intros Holdtrue.
+      apply (negb_prop_elim _ Hfalse).
+      now apply satisfied_cons_undecided. }
+    specialize (Hcover d body Hbody Holdfalse).
+    destruct Hcover as [Habs|[[v Hin]|Hd]].
+    + contradiction.
+    + destruct (Nat.eq_dec (literal_var l) v) as [->|Hneq].
+      * now left.
+      * right. left. exists v. apply ClauseMap.find_remove.
+        split; [exact Hin|congruence].
+    + now right; right.
+  - intros d Hd. destruct (Hfals d Hd) as [body [Hbody Hsem]].
+    exists body. split; [exact Hbody|].
+    now apply falsified_cons_undecided.
+  - intros v d Hin. apply ClauseMap.find_remove in Hin as [Hin Hneq].
+    destruct (Hwatch v d Hin) as [body [Hbody [Hnotin Hinc]]].
+    exists body. repeat split; try assumption.
+    intros Hin'. apply Hnotin. now apply (InL_cons_other l m v Hneq).
+  - intros v. cbn [state_watched]. rewrite ClauseMap.find_remove_eq.
+    destruct (VarKey.eq_dec (literal_var l) v); [constructor|apply Hnodup].
+  - apply Hnodup.
+  - intros d Hd. destruct (Hwatch (literal_var l) d Hd)
+      as [body [Hbody _]]. now exists body.
+  - intros p d Hpd. destruct (Hpending p d Hpd)
+      as [body [Hbody [Hpc Hp]]].
+    exists body. repeat split; try assumption. now apply literal_pending_cons.
+  - intros d Hd.
+    pose proof (ClauseMap.card_of_remove cm d (literal_var l)) as Hremove.
+    change (ClauseMap.card_of d (ClauseMap.remove (literal_var l) cm) +
+      count_occ Nat.eq_dec (ClauseMap.find (literal_var l) cm) d =
+      ClauseMap.card_of d cm) in Hremove.
+    pose proof (count_occ_nodup_in _ d (Hnodup (literal_var l)) Hd) as Hcount.
+    specialize (Hcard d). unfold card_of_watch in *.
+    cbn -[ClauseMap.card_of] in *.
+    destruct Hcard as [Hzero|[Htwo|[Hone Hwhy]]].
+    + pose proof (ClauseMap.card_of_in cm d (literal_var l) Hd). lia.
+    + left. lia.
+    + right. split; [lia|].
+      destruct Hwhy as [Habs|[Hpendingd|Hdecided']].
+      * contradiction.
+      * now left.
+      * right. now apply Hdecided.
+  - intros d.
+    pose proof (ClauseMap.card_of_remove cm d (literal_var l)) as Hremove.
+    change (ClauseMap.card_of d (ClauseMap.remove (literal_var l) cm) +
+      count_occ Nat.eq_dec (ClauseMap.find (literal_var l) cm) d =
+      ClauseMap.card_of d cm) in Hremove.
+    specialize (Hcard d). unfold card_of_watch in *.
+    cbn -[ClauseMap.card_of] in *.
+    destruct (in_dec Nat.eq_dec d
+      (ClauseMap.find (literal_var l) cm)) as [Hin|Hnotin].
+    + pose proof (count_occ_nodup_in _ d (Hnodup (literal_var l)) Hin)
+        as Hcount.
+      destruct Hcard as [Hzero|[Htwo|[Hone Hwhy]]].
+      * pose proof (ClauseMap.card_of_in cm d (literal_var l) Hin). lia.
+      * right. right. split; [lia|]. now left.
+      * left. lia.
+    + pose proof (proj1 (count_occ_not_In Nat.eq_dec _ _) Hnotin) as Hcount.
+      destruct Hcard as [Hzero|[Htwo|[Hone Hwhy]]].
+      * left. lia.
+      * right. left. lia.
+      * right. right. split; [lia|].
+        destruct Hwhy as [Habs|[Hpendingd|Hdecided']].
+        -- contradiction.
+        -- right. left. exact Hpendingd.
+        -- right. right. now apply Hdecided.
+Qed.
+
+Lemma set_lit_inv : forall l s,
+  literal_is_undecided s.(state_model) l = true ->
+  state_invariant s -> state_invariant (set_lit l s).
+Proof.
+  intros l [m clauses cm fals pending] Hlu Hinv.
+  unfold set_lit. cbn [state_model state_clauses state_watched
+    state_falsified state_pending].
+  apply fold_propagate_inv. now apply prepare_set_lit_inv.
+Qed.
+
+Lemma drop_satisfied_pending_inv : forall work l ci c pending m clauses cm fals,
+  ClauseStore.find ci clauses = Some c ->
+  In l c -> Is_true (existsb (literal_is_true m) c) ->
+  staged_invariant work
+    {| state_model := m; state_clauses := clauses; state_watched := cm;
+       state_falsified := fals; state_pending := (l, ci) :: pending |} ->
+  staged_invariant work
+    {| state_model := m; state_clauses := clauses; state_watched := cm;
+       state_falsified := fals; state_pending := pending |}.
+Proof.
+  intros work l ci c pending m clauses cm fals Hfind Hlc Htrue Hinv.
+  destruct Hinv as
+    [Hcover [Hfals [Hwatch [Hnodup [Hworknodup [Hworkref
+      [Hpending [Hwork Hcard]]]]]]]].
+  assert (Hreason : forall d,
+      (exists p, In (p, d) ((l, ci) :: pending)) ->
+      (exists p, In (p, d) pending) \/
+      decided_clause d
+        {| state_model := m; state_clauses := clauses; state_watched := cm;
+           state_falsified := fals; state_pending := pending |}).
+  { intros d [p Hpd]. simpl in Hpd. destruct Hpd as [Heq|Hpd].
+    - injection Heq as <- <-. right. right. exists c. now split.
+    - left. now exists p. }
+  repeat split; try assumption.
+  - intros p d Hpd. exact (Hpending p d (or_intror Hpd)).
+  - intros d Hd. specialize (Hwork d Hd).
+    destruct Hwork as [Hone|[Hzero [Hpendingd|Hdecided]]].
+    + now left.
+    + right. split; [exact Hzero|].
+      destruct (Hreason d Hpendingd); [now left|now right].
+    + right. split; [exact Hzero|]. now right.
+  - intros d. specialize (Hcard d).
+    destruct Hcard as [Hzero|[Htwo|[Hone Hwhy]]].
+    + now left.
+    + now right; left.
+    + right; right. split; [exact Hone|].
+      destruct Hwhy as [Hdwork|[Hpendingd|Hdecided]].
+      * now left.
+      * right. destruct (Hreason d Hpendingd); [now left|now right].
+      * right. right. exact Hdecided.
+Qed.
+
+Lemma set_pending_inv : forall l ci c pending m clauses cm fals,
+  ClauseStore.find ci clauses = Some c ->
+  literal_is_undecided m l = true ->
+  state_invariant
+    {| state_model := m; state_clauses := clauses; state_watched := cm;
+       state_falsified := fals; state_pending := (l, ci) :: pending |} ->
+  state_invariant
+    (set_lit l
+      {| state_model := m; state_clauses := clauses; state_watched := cm;
+         state_falsified := fals; state_pending := pending |}).
+Proof.
+  intros l ci c pending m clauses cm fals Hfind Hlu Hinv.
+  pose proof Hinv as Hpendinginv.
+  destruct Hpendinginv as [_ [_ [_ [_ [_ [_ [Hpending _]]]]]]].
+  destruct (Hpending l ci (or_introl eq_refl))
+    as [body [Hbody [Hlc _]]].
+  cbn in Hbody.
+  rewrite Hfind in Hbody. injection Hbody as <-.
+  unfold set_lit. cbn [state_model state_clauses state_watched
+    state_falsified state_pending].
+  apply fold_propagate_inv.
+  pose proof (prepare_set_lit_inv l m clauses cm fals ((l, ci) :: pending)
+    Hlu Hinv) as Hprepared.
+  eapply drop_satisfied_pending_inv; [exact Hfind|exact Hlc| |exact Hprepared].
+  apply Is_true_eq_left. apply existsb_exists. exists l.
+  split; [exact Hlc|apply literal_is_true_cons_self].
+Qed.
+
+Lemma resolve_true_pending_inv : forall l ci c pending m clauses cm fals,
+  ClauseStore.find ci clauses = Some c ->
+  literal_is_true m l = true ->
+  state_invariant
+    {| state_model := m; state_clauses := clauses; state_watched := cm;
+       state_falsified := fals; state_pending := (l, ci) :: pending |} ->
+  state_invariant
+    {| state_model := m; state_clauses := clauses; state_watched := cm;
+       state_falsified := fals; state_pending := pending |}.
+Proof.
+  intros l ci c pending m clauses cm fals Hfind Hltrue Hinv.
+  pose proof Hinv as Hpendinginv.
+  destruct Hpendinginv as [_ [_ [_ [_ [_ [_ [Hpending _]]]]]]].
+  destruct (Hpending l ci (or_introl eq_refl))
+    as [body [Hbody [Hlc _]]].
+  cbn in Hbody.
+  rewrite Hfind in Hbody. injection Hbody as <-.
+  eapply drop_satisfied_pending_inv; [exact Hfind|exact Hlc| |exact Hinv].
+  apply Is_true_eq_left. apply existsb_exists. now exists l.
+Qed.
+
+Lemma finish_progress_inv : forall s s',
+  state_invariant s -> finish_progress s = Progress s' -> state_invariant s'.
+Proof.
+  intros [m clauses cm fals pending] s' Hinv Hfinish.
+  unfold finish_progress in Hfinish.
+  cbn [state_falsified state_clauses] in Hfinish.
+  destruct fals as [|ci fals].
+  - now injection Hfinish as <-.
+  - destruct (ClauseStore.find ci clauses); discriminate.
+Qed.
+
+Lemma progress_inv : forall s s',
+  state_invariant s -> progress s = Progress s' -> state_invariant s'.
+Proof.
+  intros [m clauses cm fals pending] s' Hinv Hprogress.
+  unfold progress in Hprogress.
+  cbn [state_pending state_model] in Hprogress.
+  destruct pending as [|[l ci] pending].
+  - apply finish_progress_inv with
+      (s := progress_state
+        {| state_model := m; state_clauses := clauses; state_watched := cm;
+           state_falsified := fals; state_pending := [] |}); [|exact Hprogress].
+    unfold progress_state. cbn [state_pending state_model state_clauses
+      state_watched state_falsified].
+    destruct (hd_error (ClauseMap.keys cm)) as [v|] eqn:Hhead.
+    + apply set_lit_inv; [|exact Hinv].
+      apply not_InL_literal_undecided.
+      assert (In v (ClauseMap.keys cm)) as Hkey.
+      { destruct (ClauseMap.keys cm) as [|x xs] eqn:Hkeys;
+          [discriminate|]. injection Hhead as <-. now left. }
+      apply <- ClauseMap.keys_complete in Hkey.
+      destruct (ClauseMap.find v cm) as [|d ds] eqn:Hfind;
+        [contradiction|].
+      destruct Hinv as [_ [_ [Hwatch _]]].
+      assert (In d (ClauseMap.find v cm)) as Hin by (rewrite Hfind; now left).
+      destruct (Hwatch v d Hin) as [body [_ [Hnotin _]]]. exact Hnotin.
+    + exact Hinv.
+  - pose proof Hinv as Hlookup.
+    destruct Hlookup as [_ [_ [_ [_ [_ [_ [Hpending _]]]]]]].
+    destruct (Hpending l ci (or_introl eq_refl))
+      as [c [Hfind [Hlc Hstatus]]]. cbn in Hfind.
+    destruct (literal_value m l) as [[|]|] eqn:Hvalue.
+    + apply finish_progress_inv with
+        (s := progress_state
+          {| state_model := m; state_clauses := clauses; state_watched := cm;
+             state_falsified := fals;
+             state_pending := (l, ci) :: pending |}); [|exact Hprogress].
+      unfold progress_state. cbn [state_pending state_model state_clauses
+        state_watched state_falsified]. rewrite Hvalue.
+      eapply resolve_true_pending_inv; [exact Hfind| |exact Hinv].
+      unfold literal_is_true. now rewrite Hvalue.
+    + cbn [state_clauses] in Hprogress. rewrite Hfind in Hprogress.
+      discriminate.
+    + apply finish_progress_inv with
+        (s := progress_state
+          {| state_model := m; state_clauses := clauses; state_watched := cm;
+             state_falsified := fals;
+             state_pending := (l, ci) :: pending |}); [|exact Hprogress].
+      unfold progress_state. cbn [state_pending state_model state_clauses
+        state_watched state_falsified]. rewrite Hvalue.
+      eapply set_pending_inv; [exact Hfind| |exact Hinv].
+      unfold literal_is_undecided. now rewrite Hvalue.
+Qed.
+
+Lemma progress_falsified_empty : forall s s',
+  progress s = Progress s' -> s'.(state_falsified) = [].
+Proof.
+  intros s s' Hprogress. unfold progress in Hprogress.
+  destruct s.(state_pending) as [|[l ci] pending].
+  - unfold finish_progress in Hprogress.
+    destruct (progress_state s) as [m clauses cm fals pending'].
+    cbn [state_falsified state_clauses] in Hprogress.
+    destruct fals as [|d fals].
+    + now injection Hprogress as <-.
+    + destruct (ClauseStore.find d clauses); discriminate.
+  - destruct (literal_value s.(state_model) l) as [[|]|] eqn:Hvalue.
+    + unfold finish_progress in Hprogress.
+      destruct (progress_state s) as [m clauses cm fals pending'].
+      cbn [state_falsified state_clauses] in Hprogress.
+      destruct fals as [|d fals].
+      * now injection Hprogress as <-.
+      * destruct (ClauseStore.find d clauses); discriminate.
+    + cbn [state_clauses] in Hprogress.
+      destruct (ClauseStore.find ci s.(state_clauses)); discriminate.
+    + unfold finish_progress in Hprogress.
+      destruct (progress_state s) as [m clauses cm fals pending'].
+      cbn [state_falsified state_clauses] in Hprogress.
+      destruct fals as [|d fals].
+      * now injection Hprogress as <-.
+      * destruct (ClauseStore.find d clauses); discriminate.
+Qed.
+
+Lemma propagate_clauses : forall ci s,
+  (propagate ci s).(state_clauses) = s.(state_clauses).
+Proof.
+  intros ci [m clauses cm fals pending]. unfold propagate. cbn.
+  destruct (ClauseStore.find ci clauses) as [c|]; [|reflexivity].
+  destruct (scan_clause m ci c cm fals); reflexivity.
+Qed.
+
+Lemma fold_propagate_clauses : forall work s,
+  (fold_left (fun s ci => propagate ci s) work s).(state_clauses) =
+  s.(state_clauses).
+Proof.
+  induction work as [|ci work IH]; intros s; [reflexivity|].
+  simpl. rewrite IH. apply propagate_clauses.
+Qed.
+
+Lemma set_lit_clauses : forall l s,
+  (set_lit l s).(state_clauses) = s.(state_clauses).
+Proof.
+  intros l [m clauses cm fals pending]. unfold set_lit. cbn.
+  apply fold_propagate_clauses.
+Qed.
+
+Lemma progress_state_clauses : forall s,
+  (progress_state s).(state_clauses) = s.(state_clauses).
+Proof.
+  intros [m clauses cm fals pending]. unfold progress_state. cbn.
+  destruct pending as [|[l ci] pending].
+  - destruct (hd_error (ClauseMap.keys cm)); [apply set_lit_clauses|reflexivity].
+  - destruct (literal_value m l) as [[|]|]; try reflexivity.
+    apply set_lit_clauses.
+Qed.
+
+Lemma progress_clauses : forall s s',
+  progress s = Progress s' -> s'.(state_clauses) = s.(state_clauses).
+Proof.
+  intros s s' Hprogress. unfold progress in Hprogress.
+  destruct s.(state_pending) as [|[l ci] pending].
+  - unfold finish_progress in Hprogress.
+    destruct (progress_state s) as [m clauses cm fals pending'] eqn:Hstate.
+    cbn [state_falsified state_clauses] in Hprogress.
+    destruct fals as [|d fals].
+    + injection Hprogress as <-. rewrite <- Hstate. apply progress_state_clauses.
+    + destruct (ClauseStore.find d clauses); discriminate.
+  - destruct (literal_value s.(state_model) l) as [[|]|] eqn:Hvalue.
+    + unfold finish_progress in Hprogress.
+      destruct (progress_state s) as [m clauses cm fals pending'] eqn:Hstate.
+      cbn [state_falsified state_clauses] in Hprogress.
+      destruct fals as [|d fals].
+      * injection Hprogress as <-. rewrite <- Hstate. apply progress_state_clauses.
+      * destruct (ClauseStore.find d clauses); discriminate.
+    + cbn [state_clauses] in Hprogress.
+      destruct (ClauseStore.find ci s.(state_clauses)); discriminate.
+    + unfold finish_progress in Hprogress.
+      destruct (progress_state s) as [m clauses cm fals pending'] eqn:Hstate.
+      cbn [state_falsified state_clauses] in Hprogress.
+      destruct fals as [|d fals].
+      * injection Hprogress as <-. rewrite <- Hstate. apply progress_state_clauses.
+      * destruct (ClauseStore.find d clauses); discriminate.
+Qed.
+
+Inductive delay_returns {A : Type} : Delay A -> A -> Prop :=
+  | delay_returns_now (x : A) : delay_returns (Now x) x
+  | delay_returns_later (d : Delay A) (x : A) :
+      delay_returns d x -> delay_returns (Later d) x.
+
+Definition satisfies_clause_store (m : SModel) (clauses : ClauseStore.t) : Prop :=
+  forall ci c, ClauseStore.find ci clauses = Some c ->
+    Is_true (satisfies_clause m c).
+
+Lemma literal_is_true_complete_model : forall m l,
+  literal_is_true m l = true ->
+  satisfies_literal (complete_model m) l = true.
+Proof.
+  intros m [v|v] Htrue.
+  - unfold literal_is_true, literal_value,
+      satisfies_literal, complete_model, lit_is_me in *. simpl in *.
+    destruct (find (fun l => literal_var l =? v) m) as [[w|w]|];
+      try discriminate; reflexivity.
+  - unfold literal_is_true, literal_value,
+      satisfies_literal, complete_model, lit_is_me in *. simpl in *.
+    destruct (find (fun l => literal_var l =? v) m) as [[w|w]|];
+      try discriminate; reflexivity.
+Qed.
+
+Lemma terminal_state_satisfies_clauses : forall s,
+  state_invariant s ->
+  s.(state_falsified) = [] ->
+  ClauseMap.keys s.(state_watched) = [] ->
+  satisfies_clause_store (complete_model s.(state_model)) s.(state_clauses).
+Proof.
+  intros s Hinv Hfalsified Hkeys ci c Hfind.
+  destruct Hinv as [Hcover _].
+  assert (Htrue : Is_true
+    (existsb (literal_is_true s.(state_model)) c)).
+  { apply negb_prop_classical. intros Hunsat.
+    specialize (Hcover ci c Hfind Hunsat).
+    destruct Hcover as [Hwork|[[v Hwatched]|Hfals]].
+    - contradiction.
+    - assert (ClauseMap.find v s.(state_watched) <> []) as Hnonempty.
+      { intros Hempty. rewrite Hempty in Hwatched. contradiction. }
+      apply ClauseMap.keys_complete in Hnonempty. now rewrite Hkeys in Hnonempty.
+    - now rewrite Hfalsified in Hfals. }
+  apply Is_true_eq_left. unfold satisfies_clause.
+  apply Is_true_eq_true in Htrue. apply existsb_exists in Htrue as [l [Hlc Hlt]].
+  apply existsb_exists. exists l. split; [exact Hlc|].
+  now apply literal_is_true_complete_model.
+Qed.
+
+Lemma rush_unfold : forall s,
+  rush s =
+    if is_empty (ClauseMap.keys s.(state_watched)) then
+      Now (inl s.(state_model))
+    else
+      match progress s with
+      | Progress s' => Later (rush s')
+      | Conflict explanation => Now (inr explanation)
+      end.
+Proof.
+  intros s.
+  transitivity
+    (match rush s with Now x => Now x | Later d => Later d end).
+  - destruct (rush s); reflexivity.
+  - cbn [rush].
+    destruct (is_empty (ClauseMap.keys s.(state_watched)));
+      [reflexivity|].
+    destruct (progress s); reflexivity.
+Qed.
+
+Lemma rush_result_model_sound : forall s result,
+  state_invariant s ->
+  s.(state_falsified) = [] ->
+  delay_returns (rush s) result ->
+  match result with
+  | inl m => satisfies_clause_store (complete_model m) s.(state_clauses)
+  | inr _ => True
+  end.
+Proof.
+  intros s result Hinv Hfalsified Hreturns.
+  remember (rush s) as d eqn:Hrush.
+  induction Hreturns as [x|d x Hreturns IH] in s, Hinv, Hfalsified, Hrush |- *.
+  - rewrite rush_unfold in Hrush.
+    destruct (ClauseMap.keys s.(state_watched)) as [|v vs] eqn:Hkeys;
+      cbn [is_empty] in Hrush.
+    + injection Hrush as ->. now apply terminal_state_satisfies_clauses.
+    + destruct (progress s) as [s'|explanation] eqn:Hprogress;
+        [discriminate|].
+      injection Hrush as ->. exact I.
+  - rewrite rush_unfold in Hrush.
+    destruct (ClauseMap.keys s.(state_watched)) as [|v vs] eqn:Hkeys;
+      cbn [is_empty] in Hrush; [discriminate|].
+    destruct (progress s) as [s'|explanation] eqn:Hprogress;
+      [|discriminate].
+    injection Hrush as ->.
+    assert (Hinv' : state_invariant s') by
+      (now apply progress_inv with (s := s)).
+    assert (Hfalsified' : s'.(state_falsified) = []) by
+      (now apply progress_falsified_empty with (s := s)).
+    specialize (IH s' Hinv' Hfalsified' eq_refl).
+    destruct x as [m|explanation]; [|exact I].
+    rewrite <- (progress_clauses s s' Hprogress). exact IH.
+Qed.
+
+Theorem rush_model_sound : forall s m,
+  state_invariant s ->
+  s.(state_falsified) = [] ->
+  delay_returns (rush s) (inl m) ->
+  satisfies_clause_store (complete_model m) s.(state_clauses).
+Proof.
+  intros s m Hinv Hfalsified Hreturns.
+  exact (rush_result_model_sound s (inl m) Hinv Hfalsified Hreturns).
 Qed.
